src/lib/poly/Kuiper.Poly.AtomicReduce.fsti
@@ -20,12 +20,15 @@ type reduce_ty
   (r : (l:nat -> layout l))
   =
   fn (ac : is_ac_w d.pure_op)
-     (n : szp{n < max_blocks})
+     (n : szp{n <= max_blocks})
      (a : array1 et (r n) { is_global a })
      (#v_a : erased (lseq et n))
-  preserves cpu ** on gpu_loc (a |-> v_a)
-  returns   r : et
-  ensures   pure (r == Kuiper.Seq.Common.seq_fold_left d.pure_op zero v_a)
+  preserves
+    cpu ** on gpu_loc (a |-> v_a)
+  returns
+    r : et
+  ensures
+    pure (r == Kuiper.Seq.Common.seq_fold_left d.pure_op zero v_a)
 
 inline_for_extraction noextract
 val reduce
