src/lib/poly/Kuiper.Poly.DotProduct.fsti
@@ -25,7 +25,7 @@ let sum
 inline_for_extraction noextract
 type dotprod_ty
   (et:Type0) {| scalar et, real_like et |} =
-  fn (lena : szp{SZ.v lena <= max_threads})
+  fn (lena : szp{lena <= max_threads})
      (a1 : vec et)
      (a2 : vec et)
      (v1 : erased (seq et))
@@ -33,15 +33,11 @@ type dotprod_ty
      (vr1 : erased (seq real))
      (vr2 : erased (seq real) {seq_approximates v1 vr1 /\ seq_approximates v2 vr2})
      (#_: squash (len v1 == SZ.v lena /\ len v2 == SZ.v lena))
-  requires
-    cpu **
-    a1 |-> v1 **
-    a2 |-> v2
-  returns dp : et
+  preserves
+    cpu ** a1 |-> v1 ** a2 |-> v2
+  returns
+    dp : et
   ensures
-    (cpu **
-    a1 |-> v1 **
-    a2 |-> v2) **
     pure (dp `approximates` sum (pmul vr1 vr2))
 
 inline_for_extraction noextract
