src/lib/poly/Kuiper.Poly.HReduce.fsti
@@ -8,20 +8,19 @@ open Kuiper.Seq.Common
 
 inline_for_extraction noextract
 type reduce_ty (et : Type0) {| scalar et, real_like et |} =
-  fn (lena : szp { lena < max_threads })
+  fn (lena : szp { lena <= max_threads })
      (a : gpu_array et lena { is_global_array a })
      (#va : erased (seq et))
      (#vr : erased (seq real){va %~ vr})
+  preserves
+    cpu
   requires
-    cpu **
     on gpu_loc (a |-> va)
   ensures (
-    cpu **
     exists* (va' : seq et{Seq.length va' > 0}).
       on gpu_loc (a |-> va') **
       pure ((va' @! 0) %~ seq_fold_left (+.) 0.0R vr)
   )
 
 inline_for_extraction noextract
-val reduce (#et:Type0) {| scalar et, real_like et |} :
-  reduce_ty et
+val reduce (#et:Type0) {| scalar et, real_like et |} : reduce_ty et
