src/lib/poly/Kuiper.Poly.Softmax.fsti
@@ -26,18 +26,19 @@ let softmax_real (s:Seq.seq real { Seq.length s > 0 }) =
 
 unfold
 type softmax_gpu_ty (et : Type0) {| floating et, real_like et, floating_real_like et |} =
-  fn (#lena : szp { lena < max_threads })
+  fn (#lena : szp { lena <= max_threads })
      (a : gpu_array et lena { is_global_array a })
      (#va : erased (seq et))
      (#ra : erased (seq real) { Seq.length ra == SizeT.v lena /\ va %~ ra /\ lena > 0 })
+  preserves
+    cpu
   requires
-    cpu **
-    (on gpu_loc (a |-> va) **
-     pure (lena <= max_blocks))
+    on gpu_loc (a |-> va) **
+    pure (lena <= max_blocks)
   ensures (
-    cpu **
-     (exists* (v':seq et). on gpu_loc (a |-> v') **
-        pure (v' %~ softmax_real ra)))
+    exists* (v':seq et).
+      on gpu_loc (a |-> v') **
+      pure (v' %~ softmax_real ra))
 
 inline_for_extraction noextract
 val softmax_gpu (#et:Type0) {| floating et, real_like et, floating_real_like et |}
@@ -45,18 +46,19 @@ val softmax_gpu (#et:Type0) {| floating et, real_like et, floating_real_like et 
 
 unfold
 type softmax_ty (et : Type0) {| floating et, real_like et |} =
-  fn (#lena : szp { lena < max_threads })
+  fn (#lena : szp { lena <= max_threads })
      (a : Vec.lvec et lena)
      (#va : erased (seq et))
      (#ra : erased (seq real) { Seq.length ra == SizeT.v lena /\ va %~ ra /\ lena > 0 })
+  preserves
+    cpu
   requires
-    cpu **
-    (a |-> va **
-     pure (lena <= max_blocks))
+    a |-> va **
+    pure (lena <= max_blocks)
   ensures (
-    cpu **
-    (exists* (v':seq et). a |-> v' **
-        pure (v' %~ softmax_real ra)))
+    exists* (v':seq et).
+      a |-> v' **
+      pure (v' %~ softmax_real ra))
 
 inline_for_extraction noextract
 val softmax (#et : Type0) {| floating et, real_like et, floating_real_like et |}
